DLCF/Typing.lean
@@ -1,1 +1,2 @@
 import DLCF.Typing.Basic
+import DLCF.Typing.Subst
